qed on transBeePL_expr_expr_spec by changing the spec and adding induction princples

cfrontend/BeePL_compiler_proofs.v
@@ -39,49 +39,51 @@ Inductive sim_bexpr_cexpr : vmap -> BeePL.expr -> Csyntax.expr -> Prop :=
                    transBeePL_value_cvalue Vunit = cv ->
                    transBeePL_type (Ptype Tunit) g = Res ct g' i' ->
                         sim_bexpr_cexpr le (BeePL.Const ConsUnit (Ptype Tunit)) (Csyntax.Eval cv ct)*)
-| sim_app : forall le e es t ce ces ct g g' i' g'' i'',
-            transBeePL_type t g = Res ct g' i' ->  
-            transBeePL_expr_exprs transBeePL_expr_expr es g' = Res ces g'' i'' ->
+| sim_app : forall le e es t ce ces ct g g' i',
             sim_bexpr_cexpr le e ce ->
+            sim_bexprs_cexprs le es ces ->
+            transBeePL_type t g = Res ct g' i' ->  
             sim_bexpr_cexpr le (BeePL.App e es t) (Csyntax.Ecall ce ces ct)
-| sim_prim_ref : forall le e t ct ce tv g g' i', 
-                 transBeePL_type t g = Res ct g' i' ->
-                 sim_bexpr_cexpr le e ce ->
-                 gensym ct = ret tv ->
-                 sim_bexpr_cexpr le (BeePL.Prim Ref (e :: nil) t) 
-                            (Csyntax.Ecomma 
-                               (Csyntax.Eassign (Csyntax.Evar tv ct) ce ct) 
-                               (Csyntax.Eaddrof (Csyntax.Evar tv ct) ct)
-                               ct)
-| sim_prim_deref : forall le e t ct ce g g' i',
+| sim_prim_ref : forall le es t ct ces tv g g' i' g'' i'',
+                transBeePL_type t g = Res ct g' i' ->
+                sim_bexprs_cexprs le es ces ->
+                gensym ct g' = Res tv g'' i'' ->
+                sim_bexpr_cexpr le (BeePL.Prim Ref es t)
+                           (Csyntax.Ecomma 
+                              (Csyntax.Eassign (Csyntax.Evar tv ct) 
+                                             (hd default_expr (exprlist_list_expr ces)) 
+                                             ct) 
+                              (Csyntax.Eaddrof (Csyntax.Evar tv ct) ct)
+                              ct)
+| sim_prim_deref : forall le es t ct ces g g' i',
                    transBeePL_type t g = Res ct g' i' ->
-                   sim_bexpr_cexpr le e ce ->
-                   sim_bexpr_cexpr le (BeePL.Prim Deref (e :: nil) t) (Csyntax.Evalof ce ct)
-| sim_prim_massgn : forall le es t ct ces g g' i' g'' i'',
+                   sim_bexprs_cexprs le es ces ->
+                   sim_bexpr_cexpr le (BeePL.Prim Deref es t) (Csyntax.Evalof (hd default_expr (exprlist_list_expr ces)) ct)
+| sim_prim_massgn : forall le es t ct ces g g' i',
                     transBeePL_type t g = Res ct g' i' ->
-                    transBeePL_expr_exprs transBeePL_expr_expr es g' = Res ces g'' i'' ->
+                    sim_bexprs_cexprs le es ces ->
                     sim_bexpr_cexpr le (BeePL.Prim Massgn es t) 
                                    (Csyntax.Eassign 
                                       (hd default_expr (exprlist_list_expr ces))
                                       (hd default_expr (tl (exprlist_list_expr ces)))
                                       ct)
-| sim_prim_uop : forall le o es t ct ces g g' i' g'' i'', 
+| sim_prim_uop : forall le o es t ct ces g g' i', 
                 transBeePL_type t g = Res ct g' i' ->
-                transBeePL_expr_exprs transBeePL_expr_expr es g' = Res ces g'' i'' ->
+                sim_bexprs_cexprs le es ces ->
                 sim_bexpr_cexpr le (BeePL.Prim (Uop o) es t) 
                                (Csyntax.Eunop o
                                   (hd default_expr (exprlist_list_expr ces))
                                   ct)
-| sim_prim_bop : forall le o es t ct ces g g' i' g'' i'',
+| sim_prim_bop : forall le o es t ct ces g g' i',
                  transBeePL_type t g = Res ct g' i' ->
-                 transBeePL_expr_exprs transBeePL_expr_expr es g' = Res ces g'' i'' ->
+                 sim_bexprs_cexprs le es ces ->
                  sim_bexpr_cexpr le (BeePL.Prim (Bop o) es t) 
                                 (Csyntax.Ebinop o
                                    (hd default_expr (exprlist_list_expr ces))
                                    (hd default_expr (tl (exprlist_list_expr ces)))
                                    ct)
-| sim_prim_run : forall le h t,
-                 sim_bexpr_cexpr le (BeePL.Prim (Run h) nil t) (Eval (Values.Vundef) Tvoid) (* Fix me *)
+| sim_prim_run : forall le es h t,
+                 sim_bexpr_cexpr le (BeePL.Prim (Run h) es t) (Eval (Values.Vundef) Tvoid) (* Fix me *)
 | sim_bind : forall le x t e e' t' ct ct' ce ce' g g' g'' i i', (* Fix me *)
              transBeePL_type t g = Res ct g' i ->
              transBeePL_type t' g' = Res ct' g'' i' ->
@@ -102,14 +104,24 @@ Inductive sim_bexpr_cexpr : vmap -> BeePL.expr -> Csyntax.expr -> Prop :=
              sim_bexpr_cexpr le (BeePL.Addr l ofs t) (Csyntax.Eloc l.(lname) ofs l.(lbitfield) ct)
 | sim_hexpr : forall le h e t, (* Fix me *)
               sim_bexpr_cexpr le (BeePL.Hexpr h e t) (Eval (Values.Vundef) Tvoid)
-| sim_eapp : forall le ef ts es t ce cts ces ct g1 g2 i2 g3 i3 g4 i4 g5 i5,
+| sim_eapp : forall le ef ts es t ce cts ces ct g1 g2 i2 g3 i3 g4 i4,
              befunction_to_cefunction ef g1 = Res ce g2 i2 ->
              transBeePL_types transBeePL_type ts g2 = Res cts g3 i3 ->  
              transBeePL_type t g3 = Res ct g4 i4 ->
-             transBeePL_expr_exprs transBeePL_expr_expr es g4 = Res ces g5 i5 ->
+             sim_bexprs_cexprs le es ces ->
              sim_bexpr_cexpr le (BeePL.Eapp ef ts es t)
-                            (Csyntax.Ebuiltin ce cts ces ct).
+                            (Csyntax.Ebuiltin ce cts ces ct)
+with sim_bexprs_cexprs : vmap -> list BeePL.expr -> Csyntax.exprlist -> Prop :=
+| sim_nil : forall vm,
+                  sim_bexprs_cexprs vm [::] Enil
+| sim_cons : forall vm e es ce ces,
+                  sim_bexpr_cexpr vm e ce ->
+                  sim_bexprs_cexprs vm es ces ->
+                  sim_bexprs_cexprs vm (e :: es) (Econs ce ces).
  
+Scheme sim_bexpr_cexpr_ind_mut := Induction for sim_bexpr_cexpr Sort Prop
+with sim_bexprs_cexprs_ind_mut := Induction for sim_bexprs_cexprs Sort Prop.
+Combined Scheme sim_bexprs_cexprs_bexpr_cexpr_ind_mut from sim_bexpr_cexpr_ind_mut, sim_bexprs_cexprs_ind_mut.
 
 (* Complete me *)  
 (* Can put the other cases that were left out/not fixed*)
@@ -125,11 +137,8 @@ Inductive sim_bexpr_cstmt : vmap -> BeePL.expr -> Csyntax.statement -> Prop :=
                  sim_bexpr_cstmt le (BeePL.Valof e t)
                                     (Csyntax.Sreturn (Some (Evalof ce ct)))*)
 | sim_var_st : forall (le:BeePL.vmap) (le':Csem.env) x t ct g g' i',
-                   transBeePL_type t g = Res ct g' i' ->
-                  (forall le' id, if isSome (le ! id) 
-                                  then (forall l, le ! id = Some (l, t) /\ le' ! id = Some (l, ct)) 
-                                  else le ! id = None /\ le' ! id = None) ->
-                sim_bexpr_cstmt le (BeePL.Var x t) (Csyntax.Sreturn (Some (Evalof (Csyntax.Evar x ct) ct)))
+                  transBeePL_type t g = Res ct g' i' ->
+                  sim_bexpr_cstmt le (BeePL.Var x t) (Csyntax.Sreturn (Some (Evalof (Csyntax.Evar x ct) ct)))
 | sim_const_int_st : forall le i t ct g g' i',
                      transBeePL_type t g = Res ct g' i' ->
                      sim_bexpr_cstmt le (BeePL.Const (ConsInt i) t) 
@@ -142,39 +151,43 @@ Inductive sim_bexpr_cstmt : vmap -> BeePL.expr -> Csyntax.statement -> Prop :=
                       transBeePL_type t g = Res ct g' i' ->
                       sim_bexpr_cstmt le (BeePL.Const ConsUnit t)
                                      (Csyntax.Sreturn (Some (Evalof (Csyntax.Eval (Values.Vint (Int.repr 0)) ct) ct)))
-| sim_app_st : forall le e es t ce ces ct g g' i' g'' i'',
+| sim_app_st : forall le e es t ce ces ct g g' i',
                transBeePL_type t g = Res ct g' i' ->
-               transBeePL_expr_exprs transBeePL_expr_expr es g' = Res ces g'' i'' ->
+               sim_bexprs_cexprs le es ces ->
                sim_bexpr_cexpr le e ce ->
                sim_bexpr_cstmt le (BeePL.App e es t)
                               (Csyntax.Sdo (Csyntax.Ecall ce ces ct))
-| sim_prim_ref_st : forall le e t ct ce tv g g' i',
+| sim_prim_ref_st : forall le es t ct ces tv g g' i' g'' i'',
                    transBeePL_type t g = Res ct g' i' ->
-                   sim_bexpr_cexpr le e ce ->
-                   gensym ct = ret tv ->
-                   sim_bexpr_cstmt le (BeePL.Prim Ref (e :: nil) t)
+                   sim_bexprs_cexprs le es ces ->
+                   gensym ct g' = Res tv g'' i'' ->
+                   sim_bexpr_cstmt le (BeePL.Prim Ref es t)
                                   (Sdo (Csyntax.Ecomma
-                                       (Csyntax.Eassign (Csyntax.Evar tv ct) ce ct)
+                                       (Csyntax.Eassign (Csyntax.Evar tv ct) (hd default_expr (exprlist_list_expr ces)) ct)
                                        (Csyntax.Eaddrof (Csyntax.Evar tv ct) ct)
                                        ct))
-| sim_prim_deref_st : forall le e t ct ce g g' i',
+| sim_prim_deref_st : forall le es t ct ces g g' i',
                      transBeePL_type t g = Res ct g' i' ->
-                     sim_bexpr_cexpr le e ce ->
-                     sim_bexpr_cstmt le (BeePL.Prim Deref (e :: nil) t) (Sdo (Csyntax.Evalof ce ct))
-| sim_prim_massgn_st : forall le e1 e2 t ce1 ce2 ct g g' i',
+                     sim_bexprs_cexprs le es ces ->
+                     sim_bexpr_cstmt le (BeePL.Prim Deref es t) (Sdo (Csyntax.Evalof (hd default_expr (exprlist_list_expr ces)) ct))
+| sim_prim_massgn_st : forall le es t ces ct g g' i',
                        transBeePL_type t g = Res ct g' i' ->
-                       sim_bexpr_cexpr le e1 ce1 ->
-                       sim_bexpr_cexpr le e2 ce2 ->
-                       sim_bexpr_cstmt le (BeePL.Prim Massgn (e1 :: e2 :: nil) t) (Sdo (Csyntax.Eassign ce1 ce2 ct))
-| sim_prim_uop_st : forall le o e1 t ct ce1 g g' i', 
+                       sim_bexprs_cexprs le es ces ->
+                       sim_bexpr_cstmt le (BeePL.Prim Massgn es t) (Sdo (Csyntax.Eassign
+                                                                        (hd default_expr (exprlist_list_expr ces))
+                                                                        (hd default_expr (tl (exprlist_list_expr ces)))
+                                                                        ct))
+| sim_prim_uop_st : forall le o es t ct ces g g' i', 
                     transBeePL_type t g = Res ct g' i' ->
-                    sim_bexpr_cexpr le e1 ce1 ->
-                    sim_bexpr_cstmt le (BeePL.Prim (Uop o) (e1 :: nil) t) (Sdo (Csyntax.Eunop o ce1 ct))
-| sim_prim_bop_st : forall le o e1 e2 t ct ce1 ce2 g g' i',
+                    sim_bexprs_cexprs le es ces ->
+                    sim_bexpr_cstmt le (BeePL.Prim (Uop o) es t) (Sdo (Csyntax.Eunop o (hd default_expr (exprlist_list_expr ces)) ct))
+| sim_prim_bop_st : forall le o es t ct ces g g' i',
                     transBeePL_type t g = Res ct g' i' ->
-                    sim_bexpr_cexpr le e1 ce1 ->
-                    sim_bexpr_cexpr le e2 ce2 ->
-                    sim_bexpr_cstmt le (BeePL.Prim (Bop o) (e1 :: e2 :: nil) t) (Sdo (Csyntax.Ebinop o ce1 ce2 ct))
+                    sim_bexprs_cexprs le es ces ->
+                    sim_bexpr_cstmt le (BeePL.Prim (Bop o) es t) (Sdo (Csyntax.Ebinop o 
+                                                                      (hd default_expr (exprlist_list_expr ces))
+                                                                      (hd default_expr (tl (exprlist_list_expr ces)))
+                                                                      ct))
 | sim_prim_run_st : forall le h t,
                     sim_bexpr_cstmt le (BeePL.Prim (Run h) nil t) (Sdo (Eval (Values.Vundef) Tvoid)) (* Fix me *)
 | sim_bind_var_st : forall le x t e x' t' ct ct' rt ce ce' g g' i' g'' i'' g''' i''',
@@ -239,11 +252,11 @@ Inductive sim_bexpr_cstmt : vmap -> BeePL.expr -> Csyntax.statement -> Prop :=
                 sim_bexpr_cstmt le (BeePL.Addr l ofs t) (Csyntax.Sdo (Csyntax.Eloc l.(lname) ofs l.(lbitfield) ct))
 | sim_hexpr_st : forall le h e t, (* Fix me *)
                  sim_bexpr_cstmt le (BeePL.Hexpr h e t) (Sdo (Eval (Values.Vundef) Tvoid))
-| sim_eapp_st : forall le ef ts es t ce cts ces ct g1 g2 i2 g3 i3 g4 i4 g5 i5,
+| sim_eapp_st : forall le ef ts es t ce cts ces ct g1 g2 i2 g3 i3 g4 i4,
                befunction_to_cefunction ef g1 = Res ce g2 i2 ->
                transBeePL_types transBeePL_type ts g2 = Res cts g3 i3 ->
                transBeePL_type t g3 = Res ct g4 i4 ->
-               transBeePL_expr_exprs transBeePL_expr_expr es g4 = Res ces g5 i5 ->
+               sim_bexprs_cexprs le es ces ->
                sim_bexpr_cstmt le (BeePL.Eapp ef ts es t)
                               (Csyntax.Sdo (Csyntax.Ebuiltin ce cts ces ct)).
 
@@ -520,14 +533,23 @@ Qed.
 
 (***** End of Proof for correctness of type transformation *****)
 
-
-Lemma tranBeePL_expr_expr_spec: forall vm e ce g g' i,
-transBeePL_expr_expr e g = Res ce g' i ->
-sim_bexpr_cexpr vm e ce.
+Lemma transBeePL_expr_expr_spec: forall vm,
+(forall e ce g g' i,
+  transBeePL_expr_expr e g = Res ce g' i ->
+  sim_bexpr_cexpr vm e ce) /\
+(forall es ces g g' i,
+  transBeePL_expr_exprs transBeePL_expr_expr es g = Res ces g' i ->
+  sim_bexprs_cexprs vm es ces).
 Proof.
-  intro vm. induction e; intros; simpl in H.
+  intro vm. 
+  apply expr_list_expr_ind_mut with
+    (Pe := fun e => forall ce g g' i, transBeePL_expr_expr e g = Res ce g' i -> sim_bexpr_cexpr vm e ce)
+    (Pl := fun es => forall ces g g' i, transBeePL_expr_exprs transBeePL_expr_expr es g = Res ces g' i -> sim_bexprs_cexprs vm es ces);
+  intros;
+  simpl in *.
   (* Val *)
-  - unfold SimplExpr.bind in H.
+  - 
+    unfold SimplExpr.bind in H.
     destruct (transBeePL_type t g) as [| ct g1 i1] eqn:Htype; try discriminate.
     destruct (ret (Eval (transBeePL_value_cvalue v) ct) g1) as [| cs g2 i2] eqn:Hret; try discriminate.
     inversion Hret. subst cs.
@@ -536,7 +558,7 @@ Proof.
   (* Var *)
   - unfold SimplExpr.bind in H.
     destruct (transBeePL_type t g) as [| ct g1 i1] eqn:Htype; try discriminate.
-    destruct (ret (Csyntax.Evar i ct) g1) as [| cs g2 i2] eqn:Hret; try discriminate.
+    destruct (ret (Csyntax.Evar x ct) g1) as [| cs g2 i2] eqn:Hret; try discriminate.
     inversion Hret. subst cs.
     injection H as H; subst.
     eapply sim_var; eauto.
@@ -546,7 +568,7 @@ Proof.
     + destruct (transBeePL_type t g) as [| ct g1 i1] eqn:Htype; try discriminate.
       destruct (ret (Eval (Values.Vint i0) ct) g1) as [| cs g2 i2] eqn:Hret; try discriminate.
       inversion Hret. subst cs.
-      injection H as H; subst.
+      injection H as H. subst.
       eapply sim_const_int; eauto.
     + destruct (transBeePL_type t g) as [| ct g1 i1] eqn:Htype; try discriminate.
       destruct (ret (Eval (Values.Vlong i0) ct) g1) as [| cs g2 i2] eqn:Hret; try discriminate.
@@ -559,20 +581,18 @@ Proof.
       injection H as H; subst.
       eapply sim_const_unit; eauto.
   (* App *)
-  - unfold SimplExpr.bind in H.
+  - unfold SimplExpr.bind in H1.
     destruct (transBeePL_expr_expr e g) as [|cexpr g1 i1] eqn:Hexpr; try discriminate.
-    destruct (transBeePL_expr_exprs transBeePL_expr_expr l g1) as [|cexprs g2 i2] eqn:Hexprs; try discriminate.
+    destruct (transBeePL_expr_exprs transBeePL_expr_expr es g1) as [|cexprs g2 i2] eqn:Hexprs; try discriminate.
     destruct (transBeePL_type t g2) as [|ct g3 i3] eqn:Htype; try discriminate.
     destruct (ret (Ecall cexpr cexprs ct) g3) as [|cs g4 i4] eqn:Hret; try discriminate.
     inversion Hret. subst cs.
-    injection H as H. subst.
+    injection H1 as H1. subst.
     eapply sim_app; eauto.
-    (* apply Hexprs. *)
-    admit.
   (* Prim *)
-  - destruct b eqn:Hprim; unfold SimplExpr.bind in H. 
+  - destruct b eqn:Hprim; unfold SimplExpr.bind in H0. 
     (* Ref *)
-    + destruct (transBeePL_expr_exprs transBeePL_expr_expr l g) as [|cexprs g1 i1] eqn:Hexprs; try discriminate.
+    + destruct (transBeePL_expr_exprs transBeePL_expr_expr es g) as [|cexprs g1 i1] eqn:Hexprs; try discriminate.
       destruct (transBeePL_type t g1) as [|ct g2 i2] eqn:Htype; try discriminate.
       destruct (gensym ct g2) as [|i0 g3 p] eqn:Hgen; try discriminate.
       destruct (ret (Csyntax.Ecomma (Csyntax.Eassign (Csyntax.Evar i0 ct) (hd default_expr (exprlist_list_expr cexprs)) ct)
@@ -580,70 +600,65 @@ Proof.
                                     ct) g3) as [|cs g4 i4] eqn:Hret; 
                                     try discriminate.
       inversion Hret. subst cs.
-      injection H as H; subst.
-      (* eapply sim_prim_ref; eauto. *)
-      admit.
+      injection H0 as H0. subst.
+      eapply sim_prim_ref; eauto.
     (* Deref *)
-    + destruct (transBeePL_expr_exprs transBeePL_expr_expr l g) as [|cexprs g1 i1] eqn:Hexprs; try discriminate.
+    + destruct (transBeePL_expr_exprs transBeePL_expr_expr es g) as [|cexprs g1 i1] eqn:Hexprs; try discriminate.
       destruct (transBeePL_type t g1) as [| ct g2 i2] eqn:Htype; try discriminate.
       destruct (ret (Csyntax.Evalof (hd default_expr (exprlist_list_expr cexprs)) ct) g2) as [|cs g3 i3] eqn:Hret; 
       try discriminate.
       inversion Hret. subst cs.
-      injection H as H; subst.
-      (* eapply sim_prim_deref; eauto. *)
-      admit.
+      injection H0 as H0; subst.
+      eapply sim_prim_deref; eauto.
     (* Massgn *)
-    + destruct (transBeePL_expr_exprs transBeePL_expr_expr l g) as [|cexprs g1 i1] eqn:Hexprs; try discriminate.
+    + destruct (transBeePL_expr_exprs transBeePL_expr_expr es g) as [|cexprs g1 i1] eqn:Hexprs; try discriminate.
       destruct (transBeePL_type t g1) as [| ct g2 i2] eqn:Htype; try discriminate.
       destruct (ret (Csyntax.Eassign (hd default_expr (exprlist_list_expr cexprs)) 
                 (hd default_expr (tl (exprlist_list_expr cexprs))) ct) g2) as [| cs g3 i3] eqn:Hret; 
                 try discriminate.
       inversion Hret. subst cs.
-      injection H as H; subst.
-      (* eapply sim_prim_massgn; eauto. *)
-      admit.
+      injection H0 as H0; subst.
+      eapply sim_prim_massgn; eauto.
     (* Uop *)
-    + destruct (transBeePL_expr_exprs transBeePL_expr_expr l g) as [|cexprs g1 i1] eqn:Hexprs; try discriminate.
+    + destruct (transBeePL_expr_exprs transBeePL_expr_expr es g) as [|cexprs g1 i1] eqn:Hexprs; try discriminate.
       destruct (transBeePL_type t g1) as [| ct g2 i2] eqn:Htype; try discriminate.
       destruct (ret (Csyntax.Eunop u (hd default_expr (exprlist_list_expr cexprs)) ct) g2) as [| cs g3 i3] eqn:Hret;
       try discriminate.
       inversion Hret. subst cs.
-      injection H as H; subst.
-      (* eapply sim_prim_uop; eauto. *)
-      admit.
+      injection H0 as H0; subst.
+      eapply sim_prim_uop; eauto.
     (* Bop *)
-    + destruct (transBeePL_expr_exprs transBeePL_expr_expr l g) as [|cexprs g1 i1] eqn:Hexprs; try discriminate.
+    + destruct (transBeePL_expr_exprs transBeePL_expr_expr es g) as [|cexprs g1 i1] eqn:Hexprs; try discriminate.
       destruct (transBeePL_type t g1) as [| ct g2 i2] eqn:Htype; try discriminate.
       destruct (ret (Csyntax.Ebinop b0 (hd default_expr (exprlist_list_expr cexprs))
                 (hd default_expr (tl (exprlist_list_expr cexprs))) ct) g2) as [| cs g3 i3] eqn:Hret;
                 try discriminate.
       inversion Hret. subst cs.
-      injection H as H; subst.
-      (* eapply sim_prim_bop; eauto. *)
-      admit.
-    (* Run *)
-    + admit.
+      injection H0 as H0; subst.
+      eapply sim_prim_bop; eauto.
+    (* Run: Fix me *)
+    + inv H0.
+      eapply sim_prim_run.
   (* Bind *)
-  - unfold SimplExpr.bind in H.
+  - unfold SimplExpr.bind in H1.
     destruct (transBeePL_type t g) as [| ct g1 i1] eqn:Htype; try discriminate.
-    destruct (transBeePL_expr_expr e1 g1) as [| ce' g2 i2] eqn:Hexpr; try discriminate.
-    destruct (transBeePL_expr_expr e2 g2) as [| ce'' g3 i3] eqn:Hexpr'; try discriminate.
-    destruct (transBeePL_type t0 g3) as [| ct' g4 i4] eqn:Htype'; try discriminate.
-    destruct (ret (Csyntax.Ecomma (Csyntax.Eassign (Csyntax.Evar i ct) ce' ct) ce'' ct') g4) as [| cs g5 i5] eqn:Hret;
+    destruct (transBeePL_type t' g1) as [| ct' g2 i2] eqn:Htype'; try discriminate.
+    destruct (transBeePL_expr_expr e g2) as [| ce' g3 i3] eqn:Hexpr; try discriminate.
+    destruct (transBeePL_expr_expr e' g3) as [| ce'' g4 i4] eqn:Hexpr'; try discriminate.
+    destruct (ret (Csyntax.Ecomma (Csyntax.Eassign (Csyntax.Evar x ct) ce' ct) ce'' ct') g4) as [| cs g5 i5] eqn:Hret;
     try discriminate.
     inversion Hret. subst cs.
-    injection H as H; subst.
+    injection H1 as H1; subst.
     eapply sim_bind; eauto.
-    admit.
   (* Cond *)
-  - unfold SimplExpr.bind in H.
+  - unfold SimplExpr.bind in H2.
     destruct (transBeePL_expr_expr e1 g) as [| ce1 g1 i1] eqn:Hexpr1; try discriminate.
     destruct (transBeePL_expr_expr e2 g1) as [| ce2 g2 i2] eqn:Hexpr2; try discriminate.
     destruct (transBeePL_expr_expr e3 g2) as [| ce3 g3 i3] eqn:Hexpr3; try discriminate.
     destruct (transBeePL_type t g3) as [| ct g4 i4] eqn:Htype; try discriminate.
     destruct (ret (Csyntax.Econdition ce1 ce2 ce3 ct) g4) as [| cs g5 i5] eqn:Hret; try discriminate.
     inversion Hret. subst cs.
-    injection H as H; subst.
+    injection H2 as H2; subst.
     eapply sim_cond; eauto.
   (* Unit *)
   - unfold SimplExpr.bind in H.
@@ -655,30 +670,42 @@ Proof.
   (* Addr *)
   - unfold SimplExpr.bind in H.
     destruct (transBeePL_type t g) as [| ct g1 i1] eqn:Htype; try discriminate.
-    destruct (ret (Eloc (lname l) i (lbitfield l) ct) g1) as [| cs g2 i2] eqn:Hret; try discriminate.
+    destruct (ret (Eloc (lname l) ofs (lbitfield l) ct) g1) as [| cs g2 i2] eqn:Hret; try discriminate.
     inversion Hret. subst cs.
     injection H as H; subst.
     eapply sim_addr; eauto.
-  (* Hexpr *)
-  - admit.
+  (* Hexpr: Fix me*)
+  - inv H0.
+    eapply sim_hexpr.
   (* Eapp *)
-  - unfold SimplExpr.bind in H.
-    destruct (befunction_to_cefunction e g) as [| ce' g1 i1] eqn:Hfun; try discriminate.
-    destruct (transBeePL_types transBeePL_type l g1) as [| cts g2 i2] eqn:Htypes; try discriminate.
+  - unfold SimplExpr.bind in H0.
+    destruct (befunction_to_cefunction ef g) as [| ce' g1 i1] eqn:Hfun; try discriminate.
+    destruct (transBeePL_types transBeePL_type ts g1) as [| cts g2 i2] eqn:Htypes; try discriminate.
     destruct (transBeePL_type t g2) as [| ct g3 i3] eqn:Htype; try discriminate.
-    destruct (transBeePL_expr_exprs transBeePL_expr_expr l0 g3) as [| ces g4 i4] eqn:Hexprs; try discriminate.
+    destruct (transBeePL_expr_exprs transBeePL_expr_expr es g3) as [| ces g4 i4] eqn:Hexprs; try discriminate.
     destruct (ret (Ebuiltin ce' cts ces ct) g4) as [| cs g5 i5] eqn:Hret; try discriminate.
     inversion Hret. subst cs.
-    injection H as H; subst.
-    (* eapply sim_eapp; eauto. *)
-    admit.
-Admitted.
+    injection H0 as H0; subst.
+    eapply sim_eapp; eauto.
+  (* Nil *)
+  - inv H.
+    apply sim_nil.
+  - unfold SimplExpr.bind in H1.
+    destruct (transBeePL_expr_expr e g) as [| ce g1 i1] eqn:Hexpr; try discriminate.
+    destruct (transBeePL_expr_exprs transBeePL_expr_expr es g1) as [| ces' g2 i2] eqn:Hexprs; try discriminate.
+    destruct (ret (Econs ce ces') g2) as [| cs g3 i3] eqn:Hret; try discriminate. 
+    inversion Hret. subst cs.
+    injection H1 as H1; subst.
+    eapply sim_cons; eauto.
+Qed.
 
 Lemma transBeePL_expr_stmt_spec: forall vm e ce g g' i,
 transBeePL_expr_st e g = Res ce g' i ->
 sim_bexpr_cstmt vm e ce.
 Proof.
-  intro vm. induction e; intros; simpl in H.
+  intro vm. 
+  destruct transBeePL_expr_expr_spec with (vm:=vm).
+  induction e; intros; simpl in H.
   (* Val *)
   - unfold SimplExpr.bind in H.
     destruct (transBeePL_type t g) as [| ct g1 i1] eqn:Htype; try discriminate.
@@ -693,9 +720,6 @@ Proof.
     inversion Hret. subst cs.
     injection H as H. subst.
     eapply sim_var_st with (le:=vm); eauto.
-    intros. destruct (isSome (vm ! id)) eqn:His.
-    + admit.
-    + admit.
   (* Const *)
   - destruct c; unfold SimplExpr.bind in H.
     (* ConsInt *)
@@ -713,9 +737,7 @@ Proof.
       destruct (ret (Csyntax.Sreturn (Some (Evalof (Eval (transBeePL_value_cvalue Vunit) ct) ct))) g1) as [|cs g2 i2] eqn:Hret; try discriminate.
       inversion Hret. subst cs.
       injection H as H; subst.
-      admit.
-      (* eapply sim_const_unit_st with (le:=vm) (ct:=ct) (cv:=transBeePL_value_cvalue Vunit); eauto.*)
-      (* Need t := Ptype Tunit *)
+      eapply sim_const_unit_st; eauto.
   (* App *)
   - unfold SimplExpr.bind in H.
     destruct (transBeePL_expr_expr e g) as [|cexpr g1 i1] eqn:Hexpr; try discriminate.
@@ -725,6 +747,7 @@ Proof.
     inversion Hret. subst cs.
     injection H as H; subst.
     eapply sim_app_st; eauto.
+    apply transBeePL_expr_expr_spec with (vm:=vm).
     (* apply Hexprs. *)
     admit. admit.
   (* Prim *)
